Refactor some proofs out of Parameterizer. Verify automated cmp_pre checker

src/Pyrosome/Tools/Resolution.v
@@ -5,7 +5,8 @@ Import ListNotations.
 Open Scope string.
 Open Scope list.
 From Utils Require Import Utils.
-From Pyrosome Require Import Theory.Core Tools.AllConstructors Compilers.Compilers
+From Pyrosome Require Import Theory.Core Tools.AllConstructors
+  Compilers.Compilers Compilers.CompilerFacts
   Elab.Elab Elab.ElabCompilers.
 Import Core.Notations.
 (*TODO: repackage this in compilers*)
@@ -162,29 +163,6 @@ Section WithVar.
       (* should be None iff rule is an equation *)
       entry_case : option compiler_case;
     }.
-
-  
-  (*TODO: move to CompilerDefs.v*)
-  Instance compiler_case_eqb : Eqb compiler_case :=
-    fun c1 c2 =>
-      match c1, c2 with
-      | term_case args e, term_case args' e' => (eqb args args') && (eqb e e')
-      | sort_case args t, sort_case args' t' => (eqb args args') && (eqb t t')
-      | _, _ => false
-      end.
-
-  Instance compiler_case_eqb_ok : Eqb_ok compiler_case_eqb.
-  Proof.
-    intros a b;
-      destruct a, b;
-      cbn; try congruence.
-    all: lazymatch goal with
-         | |- if eqb ?x ?y && eqb ?v ?w then _ else _ =>
-             eqb_case x y;
-             eqb_case v w;
-             eauto; try congruence
-         end.
-  Qed.
     
   Section WithCompilerDb.    
     Context (db : named_list compiler_db_entry).
@@ -199,6 +177,8 @@ Section WithVar.
           && (eqb mc entry.(entry_case))
           && (inclb entry.(entry_tgt) tgt)
           && (inclb entry.(entry_cmp_pre) cmp_pre)
+          && (freshb n entry.(entry_cmp_pre))
+          && (all_freshb entry.(entry_cmp_pre))
       | None => false
       end.
 
@@ -210,21 +190,25 @@ Section WithVar.
       | term_eq_rule x x0 x1 _ => true
       end.
 
-    Fixpoint cmp_wf_in_db cmp_pre cmp src :=
+    Fixpoint cmp_wf_in_db' cmp_pre cmp src :=
       match src with
-      | [] => true
+      | [] => eqb cmp []
       | (n,r)::src' =>
           if rule_is_eqn r
           then (case_wf_in_db (cmp++cmp_pre) n r None)
-               && (cmp_wf_in_db cmp_pre cmp src')
+               && (cmp_wf_in_db' cmp_pre cmp src')
           else match cmp with
                | [] => false
                | (n', cc)::cmp' =>
                    (eqb n n')
                    && (case_wf_in_db (cmp++cmp_pre) n r (Some cc))
-                   && (cmp_wf_in_db cmp_pre cmp' src')
+                   && (cmp_wf_in_db' cmp_pre cmp' src')
                end
       end.
+    
+    Definition cmp_wf_in_db cmp_pre cmp src :=
+      (cmp_wf_in_db'  cmp_pre cmp src )
+      && (all_freshb (cmp++cmp_pre)).
 
     (*TODO: move to utils*)
     Definition option_to_list {A} ma : list A :=
@@ -235,7 +219,10 @@ Section WithVar.
         (tgt_Model := core_model e.(entry_tgt))
         e.(entry_cmp_pre)
             (map (pair n) (option_to_list e.(entry_case)))
-            [(n,e.(entry_rule))].
+            [(n,e.(entry_rule))]
+      /\ AllConstructors.all_constructors_rule
+           (fun n0 : V => In n0 (map fst e.(entry_cmp_pre)))
+           e.(entry_rule).
     
     Definition cmp_db_sound :=
       all_fresh db
@@ -243,11 +230,374 @@ Section WithVar.
       /\ all wf_entry db.
 
   End WithCompilerDb.
+    
+  Lemma empty_cmp_db_sound : cmp_db_sound [].
+  Proof.
+    unfold cmp_db_sound.
+    basic_goal_prep;
+      intuition eauto.
+  Qed.
+
+    (*TODO: move to CompilerFacts*)
+  Lemma compile_strengthen_ctx_incl (cmp1 cmp2 : compiler) c
+    : all_fresh cmp1 ->
+      all_fresh cmp2 ->
+      incl cmp1 cmp2 ->
+      AllConstructors.all_constructors_ctx (fun n0 : V => In n0 (map fst cmp1)) c ->
+      compile_ctx cmp1 c = compile_ctx cmp2 c.
+  Proof.
+    intros ? ? ?.
+    induction c;
+      basic_goal_prep;
+      eauto.
+    erewrite compile_strengthen_sort_incl;
+      auto;
+      try eassumption;
+      basic_core_crush.
+  Qed.
+
+  Definition empty_cmp_dbP := exist _ _ empty_cmp_db_sound.
+
+  Hint Resolve use_compute_all_fresh : utils.
+    
+
+  Lemma cmp_wf_in_db_correct db tgt cmp_pre cmp src
+    : cmp_db_sound db ->
+      Is_true(cmp_wf_in_db db tgt cmp_pre cmp src) ->
+      preserving_compiler_ext (tgt_Model:=core_model tgt) cmp_pre cmp src.
+  Proof.
+    unfold cmp_db_sound, cmp_wf_in_db.
+    intro Hdb.
+    autorewrite with bool utils.
+    revert cmp.
+    induction src;
+      basic_goal_prep.
+    1: basic_core_crush.
+    unfold case_wf_in_db in *.
+    revert H; destruct r; cbn; repeat case_match;
+      basic_goal_prep; subst; intuition eauto.
+    all: basic_utils_crush.
+    1,2: destruct c0, c1; basic_goal_prep.
+    5,6: destruct c; basic_goal_prep; subst.
+    1,2: destruct entry_case0.
+    all: lazymatch goal with
+         | H : Some _ = named_list_lookup_err ?db _,
+           Hall: all wf_entry ?db |-_=>
+             apply named_list_lookup_err_in in H;
+             eapply in_all in H; eauto;
+             unfold wf_entry in H;
+             cbn in *;
+             basic_core_crush;
+             try safe_invert H
+         end.
+    all: cbn in *;
+      try lazymatch goal with
+        | H : preserving_compiler_ext _ (_::_) (_::_) |-_=>
+            try safe_invert H
+        | H : preserving_compiler_ext _ [] (_::_) |-_=>
+            try safe_invert H
+           end.
+    all: try econstructor; eauto.
+    all: basic_goal_prep;basic_core_crush.
+    (*TODO: make rewrites *)
+    all: repeat lazymatch goal with
+            | H : Is_true (freshb _ _) |- _ =>
+               eapply use_compute_fresh in H
+            | H : Is_true (all_freshb _) |- _ =>
+               eapply use_compute_all_fresh in H
+            | H : Is_true (inclb _ _) |- _ =>
+               eapply use_inclb in H               
+           end.
+    {
+      eapply wf_sort_lang_monotonicity; eauto.
+      erewrite <- compile_strengthen_ctx_incl; [eassumption| ..];
+        eauto.
+      all: basic_utils_crush.
+      intros [x c] Hin.
+      assert (x <> v1).
+      {
+        intro; subst.
+        basic_utils_crush.
+      }                    
+      eapply H12 in Hin.
+      basic_goal_prep;basic_core_crush.
+    }
+    {
+      eapply wf_term_lang_monotonicity; eauto.
+      erewrite <- compile_strengthen_sort_incl,
+         <- compile_strengthen_ctx_incl;
+        [eassumption| ..];
+        eauto.
+      all: basic_utils_crush.
+      all:intros [x c] Hin;
+      assert (x <> v1) by (basic_goal_prep;basic_core_crush).                   
+      all:eapply H12 in Hin; basic_goal_prep;basic_core_crush.
+    }
+    {
+      eapply eq_sort_lang_monotonicity; eauto.
+      erewrite <- compile_strengthen_sort_incl,
+         <- compile_strengthen_ctx_incl; eauto.
+      1:erewrite <- compile_strengthen_sort_incl with (t:=s2); eauto.
+    }
+    {
+      eapply eq_term_lang_monotonicity; eauto.
+      erewrite <- compile_strengthen_sort_incl,
+         <- compile_strengthen_incl,
+         <- compile_strengthen_ctx_incl; eauto.
+      1:erewrite <- compile_strengthen_incl with (e:=t2); eauto.
+    }
+  Qed.
+  
+  Lemma cmp_db_append_sound db1 db2
+    : Is_true(all_freshb (db1++db2)) ->
+      cmp_db_sound db1 ->
+      cmp_db_sound db2 ->
+      cmp_db_sound (db1++db2).
+  Proof.
+    intro H.
+    apply use_compute_all_fresh in H.
+    unfold cmp_db_sound.
+    intuition eauto.
+    clear H H2 H0.
+    revert H3.
+    induction db1;
+      basic_goal_prep;
+      basic_core_crush.
+  Qed.
+
+  Definition cmp_dbP_append
+    (dbP1 dbP2 : { db | cmp_db_sound db })
+    (check : Is_true(all_freshb (proj1_sig dbP1 ++ proj1_sig dbP2))) : { db | cmp_db_sound db } :=
+    exist _ (proj1_sig dbP1 ++ proj1_sig dbP2)
+      (cmp_db_append_sound check (proj2_sig dbP1) (proj2_sig dbP2)).
+
+  Fixpoint cmp_to_db tgt cmp_pre (src : lang) (cmp : compiler) : named_list _ :=
+    match src with
+    | [] => []
+    | (n,r)::src' =>
+        if rule_is_eqn r
+        then (n,Build_compiler_db_entry tgt (cmp++cmp_pre) r None)
+               :: (cmp_to_db tgt cmp_pre src' cmp)
+        else match cmp with
+             | [] => [] (* never happens*)
+             | (_,cc)::cmp' =>
+                 (n,Build_compiler_db_entry tgt (cmp'++cmp_pre) r (Some cc))
+                   :: (cmp_to_db tgt cmp_pre src' cmp')
+             end
+    end.
+  
+  Lemma cmp_to_db_fresh n tgt cmp_pre src cmp
+    : fresh n src -> fresh n (cmp_to_db tgt cmp_pre src cmp).
+  Proof.
+    revert cmp;
+      induction src;
+      destruct cmp;
+      basic_goal_prep;
+      basic_core_crush.
+    all:destruct r;
+      basic_goal_prep;
+      basic_core_crush.
+  Qed.
+
+  (* TODO: move to AllCOnstructors *)
+  Fixpoint all_constructorsb (P : V -> bool) e : bool :=
+    match e with
+    | var _ => true
+    | con n s => P n && forallb (all_constructorsb P) s
+    end.
+  
+  Definition all_constructors_sortb (P : V -> bool) t : bool :=
+    match t with
+    | scon n s => P n && forallb (all_constructorsb P) s
+    end.
+
+  Notation all_constructors_ctxb P c :=
+    (forallb (fun p => all_constructors_sortb P (snd p)) c).
+  
+  Definition all_constructors_ruleb P r :=
+    match r with
+    | sort_rule c _ => all_constructors_ctxb P c
+    | term_rule c _ t => all_constructors_ctxb P c && all_constructors_sortb P t
+    | sort_eq_rule c t1 t2 =>
+        all_constructors_ctxb P c
+        && all_constructors_sortb P t1
+        && all_constructors_sortb P t2
+    | term_eq_rule c e1 e2 t =>
+        all_constructors_ctxb P c
+        && all_constructors_sortb P t
+        && all_constructorsb P e1
+        && all_constructorsb P e2
+    end.
+
+  Fixpoint all_constructors_in_lang ctrs_pre l :=
+    match l with
+    | [] => True
+    | (n,r)::l' =>
+        let l_ctrs := map fst (filter (fun x => negb (rule_is_eqn (snd x))) l') in
+        all_constructors_rule (fun n0 : V => In n0 (l_ctrs ++ ctrs_pre)) r
+        /\ all_constructors_in_lang ctrs_pre l'
+    end.
+  
+  Fixpoint all_constructors_in_langb ctrs_pre l :=
+    match l with
+    | [] => true
+    | (n,r)::l' =>
+        let l_ctrs := map fst (filter (fun x => negb (rule_is_eqn (snd x))) l') in
+        all_constructors_ruleb (fun n0 : V => inb n0 (l_ctrs++ctrs_pre)) r
+        && all_constructors_in_langb ctrs_pre l'
+    end.
+
+  
+  Lemma all_constructorsb_spec Pb P e
+    : (forall x, Is_true (Pb x) <-> P x) ->
+      Is_true (all_constructorsb Pb e) <-> all_constructors P e.
+  Proof.
+    intro Prw.
+    induction e;
+      basic_goal_prep;
+      autorewrite with utils bool;
+      try tauto.
+    rewrite Prw.
+    revert H; clear;
+      induction l;
+      basic_goal_prep;
+      basic_utils_crush.
+  Qed.
+    
+  Lemma all_constructors_sortb_spec Pb P t
+    : (forall x, Is_true (Pb x) <-> P x) ->
+      Is_true (all_constructors_sortb Pb t) <-> all_constructors_sort P t.    
+  Proof.
+    intro Prw.
+    destruct t;
+      basic_goal_prep;
+      autorewrite with utils bool;
+      try tauto.
+    rewrite Prw.
+    induction l;
+      basic_goal_prep;
+      basic_utils_crush.
+    { rewrite <- all_constructorsb_spec; eauto. }
+    { rewrite all_constructorsb_spec; eauto. }      
+  Qed.
+
+  
+    
+  Lemma all_constructors_ctxb_spec Pb (P : V -> Prop) (c : ctx)
+    : (forall x, Is_true (Pb x) <-> P x) ->
+      Is_true (all_constructors_ctxb Pb c) <-> all_constructors_ctx P c.    
+  Proof.
+    intro Prw.
+    induction c;
+      basic_goal_prep;
+      basic_utils_crush.
+    { rewrite <- all_constructors_sortb_spec; eauto. }
+    { rewrite all_constructors_sortb_spec; eauto. }      
+  Qed.
+
+  (*TODO: copied; move to lists*)
+   Lemma all_implies A (P Q : A -> Prop) l
+    : (forall x,  P x -> Q x) -> all P l -> all Q l.
+  Proof.
+      induction l;
+      basic_goal_prep;
+      basic_utils_crush.
+  Qed.
+    
+  Lemma all_constructors_ruleb_spec Pb (P : V -> Prop) (r : rule)
+    : (forall x, Is_true (Pb x) <-> P x) ->
+      Is_true (all_constructors_ruleb Pb r) <-> all_constructors_rule P r.    
+  Proof.
+    intro Prw.
+    destruct r;
+      basic_goal_prep;
+      autorewrite with utils bool in *.
+    all: rewrite ?all_constructors_ctxb_spec,
+        ?all_constructors_sortb_spec,
+        ?all_constructorsb_spec in *;
+      try eassumption.
+    all: intuition eauto.
+    all: eapply all_implies; try eassumption.
+    all: basic_goal_prep.
+    all: rewrite ?all_constructors_ctxb_spec,
+        ?all_constructors_sortb_spec,
+        ?all_constructorsb_spec in *;
+      try eassumption.
+  Qed.   
+
+  Lemma all_constructors_in_langb_spec l_pre l
+    : Is_true (all_constructors_in_langb l_pre l) <-> all_constructors_in_lang l_pre l.
+  Proof.
+    induction l;
+      basic_goal_prep;
+      try tauto.
+    autorewrite with bool utils.
+    rewrite !all_constructors_ruleb_spec,
+      !IHl.
+    1:reflexivity.
+    basic_goal_prep;
+      basic_utils_crush.
+  Qed.
+
+  
+  Lemma fst_filter_lang_cmp tgt cmp_pre cmp l
+    :  preserving_compiler_ext (tgt_Model:=core_model tgt) cmp_pre cmp l ->
+       map fst (filter (fun x : V * rule => negb (rule_is_eqn (snd x))) l)
+       = map fst cmp.
+  Proof.
+    induction 1;
+      basic_goal_prep;
+      basic_core_crush.
+  Qed.
+
+  Lemma wf_cmp_sound_db tgt cmp_pre src cmp
+    : preserving_compiler_ext (tgt_Model:=core_model tgt) cmp_pre cmp src ->
+      Is_true (all_freshb src && all_constructors_in_langb (map fst cmp_pre) src) ->
+      cmp_db_sound (cmp_to_db tgt cmp_pre src cmp).
+  Proof.
+    unfold cmp_db_sound.
+    intros H1 H2.
+    autorewrite with bool utils in *; break.
+    apply all_constructors_in_langb_spec in H0.
+    apply use_compute_all_fresh in H.
+    revert H1 H H0.
+    induction 1;
+      basic_goal_prep;
+      try tauto;
+      autorewrite with utils bool lang_core term model in *.
+    all: basic_goal_prep.
+    all: intuition eauto using cmp_to_db_fresh with lang_core.
+    all: try eapply all_implies; eauto.
+    all: basic_goal_prep.
+    all: try eapply all_constructors_sort_weaken; eauto.
+    all: try eapply all_constructors_term_weaken; eauto.
+    all: basic_goal_prep.
+    all: erewrite fst_filter_lang_cmp in *; eauto.
+    all: rewrite map_app.
+    all: eauto.
+  Qed.
+  
+  (*TODO: whole-compiler append*)
+  Definition db_append_cmp tgt cmp_pre cmp src
+    (wfc : preserving_compiler_ext (tgt_Model:=core_model tgt) cmp_pre cmp src)
+    (checks : Is_true (all_freshb src && all_constructors_in_langb (map fst cmp_pre) src))
+    (dbP2 : { db | cmp_db_sound db }) :=
+    let db1 := (cmp_to_db tgt cmp_pre src cmp) in
+    let pf1 := wf_cmp_sound_db wfc checks in 
+    fun (check : Is_true(all_freshb (db1 ++ proj1_sig dbP2))) =>
+      exist _ (db1 ++ proj1_sig dbP2)
+        (cmp_db_append_sound check pf1 (proj2_sig dbP2)).
+
   
 End WithVar.
   
 Ltac prove_by_lang_db dbP :=
   apply (lang_wf_in_db_correct _ _ (proj2_sig dbP));
+  vm_compute; exact I.
+
+
+Ltac prove_by_cmp_db dbP :=
+  apply (cmp_wf_in_db_correct _ _ (proj2_sig dbP));
   vm_compute; exact I.
 
 (*TODO: this doesn't work since if 2 files overwrite it, importing 1 will erase the other*)
